Cleanup RC_DC.

Common/Rc_dynamic.v
@@ -4,29 +4,29 @@ Require Import CompCert.Behaviors.
 Require Import Coq.Lists.List.
 Require Import Coq.Program.Basics.
 Require Import Common.Definitions.
-Require Import Common.Linking.
-Require Import Intermediate.Machine.
-Require Import Intermediate.CS.
-Require Import Intermediate.PS.
 
 (* 
-   Full proof of robust compilation relying on 
-   - target decomposition,
-   - compiler correctness and 
+   Top-down proof of Robust Compilation Dynamic Compromise relying on 
+   - target decomposition
+   - compiler correctness 
    - source definability
-  
-   For a simple instance refer to SI.RC, a more complicate instance is
-   in Main.robust_compilation_static_compromise.
  *)
 
-(* 
-   Some Global definitions.
+(*
+  Some Global definitions.
  *)
 
 (* Component id *)
-Definition partition := list Component.id.
-Definition interface := Program.interface.
+Definition interface := list Component.id.
+(* check if an interface is complete *)
+Axiom icomplete : interface -> Prop.
+(* check if the union of two interfaces is complete *)
+Definition icomplete2 (i1 i2:interface) := icomplete (i1++i2).
+(* check if a interface is contained in another *)
+Definition contained {A} (i1 i2: list A) := exists i3, i1++i3=i2.
 
+(* A partition is less than an inteface and will simplify proofs. *)
+Definition partition := list Component.id.
 (* check if the last event of a behavior belongs to an agent,
    represented by the interface of its components *)
 Definition turn_trace (t:trace) (par:partition) : Prop :=
@@ -35,29 +35,22 @@ Definition turn_trace (t:trace) (par:partition) : Prop :=
               | ECall Cid Pid n Cid' => In Cid' par
               | ERet Cid n Cid' => In Cid' par
               end).
-  
-
-(* For now turn is defined only for finite traces. *)
+(* turn is defined only for finite traces. *)
 Definition turn (b:program_behavior) (i:partition) : Prop :=
   exists t, turn_trace t i /\
             ((exists n, b = Terminates t n) \/
             (b = Diverges t) \/
             (b = Goes_wrong t)).
-             
-  
-(* check if an interface is complete *)
-Definition icomplete := Linking.closed_interface.
-(* check if the union of two interfaces is complete *)
-Definition icomplete2 (i1 i2:interface) := icomplete (NMapExtra.update i1 i2).
-(* check if a interface is contained in another *)
-Definition contained (i1 i: interface) :=
-  exists i2, NMap.Equal (NMapExtra.update i1 i2) i.
-
-
 Definition behavior_improves_p (behs beht:program_behavior) (par:partition) :=
   (behs = beht \/ (exists t, behs = Goes_wrong t /\
                              behavior_prefix t beht /\
                              turn behs par)).
+
+Lemma behavior_improves_p_trans:
+  forall beh1 beh2 beh3 p,
+  behavior_improves_p beh1 beh2 p -> behavior_improves_p beh2 beh3 p ->
+  behavior_improves_p beh1 beh3 p.
+Proof. Admitted.
 
 (* 
    The languages.
@@ -87,20 +80,9 @@ Module Type Lang.
     valid p1 /\ valid p2 /\
     icomplete2 (get_interface p1) (get_interface p2).
 
-  (* CompCert defines the semantics of a program as an object providing the following:  
-Record semantics : Type := Semantics_gen {
-  state: Type;
-  genvtype: Type;
-  step : genvtype -> state -> trace -> state -> Prop;
-  initial_state: state -> Prop;
-  final_state: state -> int -> Prop;
-  globalenv: genvtype;
-}.
-
-   any program has a semantics, if the program is ill-formed it
-   still has a behavior. e.g. a program without any initial state
-   satisfies program_goes_initially_wrong
-   *)
+  (* In CompCert any program has a semantics, if the program is
+   ill-formed it still has a behavior. e.g. a program without any
+   initial state satisfies program_goes_initially_wrong *)
   
   (* produces a complete semantics from a complete program *)
   Parameter sem: program -> semantics.
@@ -111,59 +93,6 @@ Record semantics : Type := Semantics_gen {
   (* TODO we should check that program is complete and interface is contained *)
   Parameter psem: interface -> program -> semantics.
 
-  (* Parameter val : Type. *)
-  (* Record CoreSemantics {G C M : Type} : Type := *)
-  (* { initial_core : G -> val -> list val -> option C *)
-  (* ; at_external : C -> option (external_function * signature * list val) *)
-  (* ; after_external : val -> C -> option C *)
-  (* ; halted : C -> val *)
-  (* ; corestep : G -> C -> M -> C -> M -> Prop *)
-  (* (* plus lemmas *) *)
-  (* }. *)
-  
-  (* Parameter csem: semantics. *)
-  (* Parameter pstate : Type. *)
-  (* Parameter penv : Type. *)
-  (* Parameter turn_state : pstate -> Component.id. *)
-  (* Parameter psi: interface. *)
-  (* Parameter partialize: interface -> (state csem) -> pstate. *)
-  (* Parameter lift: interface -> pstate -> (state csem). *)
-  (* (* TODO lemma between lift and partialize *) *)
-  (* Parameter lift_env: penv -> (genvtype csem). *)
-  (* (* Parameter stack_push: pstate -> Component.id -> pstate. *) *)
-  (* Parameter is_program_component : penv -> Component.id -> Prop. *)
-  (* Parameter is_context_component : penv -> Component.id -> Prop. *)
-
-  (* Definition initial_state (ps:pstate) := initial_state csem (lift psi ps). *)
-  (* Definition final_state (ps:pstate) := final_state csem (lift psi ps). *)
-  (* Inductive pstep: penv -> pstate -> trace -> pstate -> Prop := *)
-  (* (* TODO the event can't be read *) *)
-  (* | program_all: forall g ps ps', *)
-  (*     is_program_component g (turn_state ps) -> *)
-  (*     (step csem) (lift_env g) (lift psi ps) E0 (lift psi ps') -> *)
-  (*     pstep g ps E0 ps' *)
-  (* | context_epsilon: forall g ps, *)
-  (*     is_context_component g (turn_state ps) -> *)
-  (*     Program.has_component_id psi (turn_state ps) -> *)
-  (*     pstep g ps E0 ps *)
-  (* | Context_Internal_Call: *)
-  (*     forall pgps pgps' mem C C' P call_arg, *)
-  (*       let C = turn_state(ps) in *)
-  (*       let C' = turn_state(ps') in *)
-  (*       C' <> C -> *)
-  (*       imported_procedure (genv_interface G) C C' P -> *)
-  (*       is_context_component G C -> *)
-  (*       is_context_component G C' -> *)
-  (*       pgps' = (C, None) :: pgps -> *)
-  (*       let t := [ECall C P call_arg C'] in *)
-  (*       step G (CC (pgps,mem,C)) t (CC (pgps',mem,C')). *)
-
-  (*     step G (PC (pgps,mem,regs,pc)) E0 (PC (pgps,mem',regs',pc')) *)
-             
-  (* Definition psem (psi:interface) (p:program) := *)
-  (*   Semantics_gen (step csem) (initial_state csem) (final_state csem) (globalenv csem). *)
-
-
 End Lang.
 
 (* Every language is a subtype of Lang and implements its signature *)
@@ -171,22 +100,17 @@ End Lang.
 
 (* Intermediate *)
 Module I <: Lang.
-  Axiom state: Type.
-  Axiom initial_state: state -> Prop.
-  Definition program := Intermediate.program.
-  Definition get_interface := Intermediate.prog_interface.
+  Axiom program : Type.
   Axiom valid: program -> Prop.
-
+  Axiom get_interface: program -> interface.
   Definition complete (p:program) :=
     valid p /\ icomplete (get_interface p).
   Definition complete2 (p1 p2:program) :=
     valid p1 /\ valid p2 /\
     icomplete2 (get_interface p1) (get_interface p2).
-
-  Axiom main_c : Component.id.
-  Axiom main_p : Procedure.id.
-  Definition sem p := CS.sem p main_c main_p. 
-  Definition psem (psi:interface) p := PS.sem p main_c main_p.
+    
+  Axiom sem: program -> semantics.
+  Axiom psem: interface -> program -> semantics.
 
   (* linking of two partial programs, this is restricted to the
      complete case, we could generalize by asking that p1 and p2 are
@@ -195,7 +119,7 @@ Module I <: Lang.
   Axiom link_spec:
     forall (p1 p2 p:program),
       complete2 p1 p2 ->
-      NMap.Equal (NMapExtra.update (get_interface p1) (get_interface p2)) (get_interface p) /\
+      (get_interface p1) ++ (get_interface p2) = (get_interface p) /\
       complete (link p1 p2).
 
   Axiom decomposition:
@@ -204,14 +128,10 @@ Module I <: Lang.
       program_behaves (sem (link c p)) beh ->
       program_behaves (psem (get_interface c) p) beh.
 
-  (* CH: TODO: I find the `valid` and `icomplete2` **preconditions** disturbing;
-               this makes invalid or incomplete programs fully_defined *)
 End I.
 
 (* Source *)
 Module S <: Lang.
-  Axiom state: Type.
-  Axiom initial_state: state -> Prop.
   Axiom program : Type.
   Axiom valid: program -> Prop.
   Axiom get_interface: program -> interface.
@@ -236,28 +156,24 @@ Module S <: Lang.
         program_behaves (sem (link c p)) beh.
 End S.
 
-
 (* Source to Intermediate *)
 Module SI.
-  (* TODO
-     compcert defined the compiler as:
-     - a function transf_c_program (p: Csyntax.program) : res Asm.program
-     - a relation match_prog: Csyntax.program -> Asm.program -> Prop
-     and proves their equivalence in transf_c_program_match.
- *)
   (* compiles partial programs *)
   Axiom compile : S.program -> I.program.
   Axiom compile_spec:
     forall (p:S.program),
       S.valid p ->
-      I.valid (compile p) /\
-      NMap.Equal (S.get_interface p) (I.get_interface (compile p)).
+      I.valid (compile p) /\ S.get_interface p = I.get_interface (compile p).
 
   Axiom Sreceptive:
     forall P, receptive (S.sem P).
   Axiom Ideterminate:
     forall p, determinate (I.sem p).
-  
+
+  (* In compcert there are two simulation: *)
+  (*   - forward: is just a simulation, it is forward or backward depending on the order of the arguments *)
+  (*   - backward: add the condition that the first argument must be a safe program *)
+
   Axiom complete_forward_simulation :
     forall P,
       S.complete P ->
@@ -273,7 +189,8 @@ Module SI.
     auto. auto.
     apply Sreceptive. apply Ideterminate.
   Qed.
-  
+
+  (* TODO this shoudl be improves_p *)
   Theorem complete_compiler_correctness:
     forall P behi,
       S.complete P ->
@@ -284,39 +201,19 @@ Module SI.
     apply complete_backward_simulation; auto.
   Qed.
 
-
-  Variable partial_match_states: state  -> state L2 -> Prop.
-  
-  Hypothesis partial_match_initial_states:
-    forall s1, initial_state L1 s1 ->
-               exists s2, initial_state L2 s2 /\ match_states s1 s2.
-  
-  Hypothesis partial_match_final_states:
-    forall s1 s2 r,
-      match_states s1 s2 ->
-      final_state L1 s1 r ->
-      final_state L2 s2 r.
-
-
-  (* TODO this should be provable from backward_simulation_complete *)
-  (* TODO this should backward *)
-  Definition partial_forward_simulation:
+  (* this should be provable from the complete backward simulation *)
+  Axiom partial_backward_simulation:
     forall P psi,
       S.valid P ->
       icomplete2 psi (S.get_interface P) ->
-      forward_simulation (S.psem psi P) (I.psem psi (compile P)).
-  Proof.
-    intros P psi ValP icomp.
-    eapply forward_simulation_plus.
+      backward_simulation (S.psem psi P) (I.psem psi (compile P)).
 
-
-
-  Axiom backward_simulation_behavior_improves_p:
+  Axiom partial_backward_simulation_behavior_improves_p:
     forall psi p1 p2,
       backward_simulation (S.psem psi p1) (I.psem psi p2) ->
-    forall beh2, program_behaves (I.psem psi p2) beh2 ->
-    exists beh1, program_behaves (S.psem psi p1) beh1 /\ behavior_improves_p beh1 beh2 (S.get_interface p1).
-
+    forall behi, program_behaves (I.psem psi p2) behi ->
+    exists behs, program_behaves (S.psem psi p1) behs /\ behavior_improves_p behs behi (S.get_interface p1).
+    
   Theorem partial_compiler_correctness:
     forall P psi behi,
       S.valid P ->
@@ -324,10 +221,9 @@ Module SI.
       program_behaves (I.psem psi (compile P)) behi ->
       exists behs, program_behaves (S.psem psi P) behs /\ behavior_improves_p behs behi (S.get_interface P).
   Proof.
-    intros. eapply backward_simulation_behavior_improves_p; eauto.
+    intros. eapply partial_backward_simulation_behavior_improves_p; eauto.
     apply partial_backward_simulation; auto.
   Qed.
-
 End SI.
 
 
@@ -337,8 +233,11 @@ Module MP <: Lang.
   Axiom program : Type.
   Axiom valid: program -> Prop.
   Axiom get_interface: program -> interface.
-  Definition complete (p:program) := valid p /\ icomplete (get_interface p).
-  Definition complete2 (p1 p2:program) := valid p1 /\ valid p2 /\ icomplete2 (get_interface p1) (get_interface p2).
+  Definition complete (p:program) :=
+    valid p /\ icomplete (get_interface p).
+  Definition complete2 (p1 p2:program) :=
+    valid p1 /\ valid p2 /\
+    icomplete2 (get_interface p1) (get_interface p2).
   Axiom sem: program -> semantics.
   Axiom psem: interface -> program -> semantics.
 End MP.
@@ -348,8 +247,11 @@ Module SFI <: Lang.
   Axiom program : Type.
   Axiom valid: program -> Prop.
   Axiom get_interface: program -> interface.
-  Definition complete (p:program) := valid p /\ icomplete (get_interface p).
-  Definition complete2 (p1 p2:program) := valid p1 /\ valid p2 /\ icomplete2 (get_interface p1) (get_interface p2).
+  Definition complete (p:program) :=
+    valid p /\ icomplete (get_interface p).
+  Definition complete2 (p1 p2:program) :=
+    valid p1 /\ valid p2 /\
+    icomplete2 (get_interface p1) (get_interface p2).
   Axiom sem: program -> semantics.
   Axiom psem: interface -> program -> semantics.
 End SFI.
@@ -359,13 +261,6 @@ End SFI.
    Both backend MP and SFI need to implement this interface *)
 Module Type IT.
   Declare Module T : Lang.
-  
-  (* TODO
-     compcert defines the compiler as:
-     - a function transf_c_program (p: Csyntax.program) : res Asm.program
-     - a relation match_prog: Csyntax.program -> Asm.program -> Prop
-     and proves their equivalence in transf_c_program_match.
-   *)
   (* Note that 
      - this compiler only works on complete programs as
        opposed to SI.compile that works on partial programs 
@@ -377,7 +272,7 @@ Module Type IT.
   Parameter compile_spec:
     forall (p:I.program),
       I.complete p -> T.valid (compile p) /\
-                      I.get_interface p = T.get_interface (compile p).
+                   I.get_interface p = T.get_interface (compile p).
   
   (* 
      The following properties are special because they depend on
@@ -394,10 +289,11 @@ Module Type IT.
       program_behaves (T.psem (I.get_interface c) ip) beh.
 
   Parameter special_compiler_correctness:
-    forall (behi beht:program_behavior) (c p:I.program),
+    forall (beht:program_behavior) (c p:I.program),
       I.complete2 c p ->
       let ip := I.link c p in
       program_behaves (T.psem (I.get_interface c) (compile ip)) beht ->
+      exists behi,
       program_behaves (I.psem (I.get_interface c) p) behi /\
       behavior_improves_p behi beht (I.get_interface p).
 
@@ -407,156 +303,121 @@ Module Type IT.
     forall p b, program_behaves (T.sem p) b -> not_wrong b.
 End IT.
 
-(* (* Micro-policies compiler *) *)
-(* Module MPC <: IT. *)
-(*   Module T := MP. *)
+(* Micro-policies compiler *)
+Module MPC <: IT.
+  Module T := MP.
   
-(*   Axiom compile : I.program -> T.program. *)
-(*   Axiom compile_spec: *)
-(*     forall (p:I.program), *)
-(*       I.complete p -> T.valid (compile p) /\ *)
-(*                    I.get_interface p = T.get_interface (compile p). *)
+  Axiom compile : I.program -> T.program.
+  Axiom compile_spec:
+    forall (p:I.program),
+      I.complete p -> T.valid (compile p) /\
+                   I.get_interface p = T.get_interface (compile p).
 
-(*   (* this would be used in the definition of T.psem and in match_states *) *)
-(*   (* Axiom partialize: interface -> T.program -> T.program. *) *)
-(*   (* Axiom partialize_spec: *) *)
-(*   (*   forall psi (p:T.program), *) *)
-(*   (*     T.valid p -> *) *)
-(*   (*     contained psi (T.get_interface p) -> *) *)
-(*   (*     (T.get_interface p) = (T.get_interface (partialize psi p))++psi. *) *)
+  (* this would be used in the definition of T.psem and in match_states *)
+  (* Axiom partialize: interface -> T.program -> T.program. *)
+  (* Axiom partialize_spec: *)
+  (*   forall psi (p:T.program), *)
+  (*     T.valid p -> *)
+  (*     contained psi (T.get_interface p) -> *)
+  (*     (T.get_interface p) = (T.get_interface (partialize psi p))++psi. *)
 
-(*   Axiom sem_spec: *)
-(*     forall p b, program_behaves (T.sem p) b -> not_wrong b. *)
+  Axiom sem_spec:
+    forall p b, program_behaves (T.sem p) b -> not_wrong b.
 
-(*   Axiom psem_spec: *)
-(*     forall psi p b, program_behaves (T.psem psi p) b -> not_wrong b. *)
+  Axiom psem_spec:
+    forall psi p b, program_behaves (T.psem psi p) b -> not_wrong b.
 
-(*   (* assuming we have a simulation *) *)
-(*   Axiom decomposition_simulation: *)
-(*     forall psi tp, *)
-(*     forward_simulation (T.sem tp) (T.psem psi tp). *)
+  (* assuming we have a simulation *)
+  Axiom decomposition_simulation:
+    forall psi tp,
+    forward_simulation (T.sem tp) (T.psem psi tp).
     
-(*   Definition decomposition: *)
-(*     forall beh psi (p:T.program), *)
-(*       T.valid p -> *)
-(*       contained psi (T.get_interface p) -> *)
-(*       program_behaves (T.sem p) beh -> *)
-(*       program_behaves (T.psem psi p) beh. *)
-(*   Proof. *)
-(*     intros b psi p Hvalp Hcont Hsem. *)
-(*     eapply forward_simulation_same_safe_behavior. *)
-(*     apply decomposition_simulation. *)
-(*     assumption. *)
-(*     apply (sem_spec p). *)
-(*     assumption. *)
-(*   Qed. *)
+  Definition decomposition:
+    forall beh psi (p:T.program),
+      T.valid p ->
+      contained psi (T.get_interface p) ->
+      program_behaves (T.sem p) beh ->
+      program_behaves (T.psem psi p) beh.
+  Proof.
+    intros b psi p Hvalp Hcont Hsem.
+    eapply forward_simulation_same_safe_behavior.
+    apply decomposition_simulation.
+    assumption.
+    apply (sem_spec p).
+    assumption.
+  Qed.
   
-(*   (* we can prove special decomposition using the more general *)
-(*      decomposition *) *)
-(*   Definition special_decomposition : *)
-(*     forall beh (c p:I.program), *)
-(*       I.complete2 c p -> *)
-(*       program_behaves (T.sem (compile (I.link c p))) beh -> *)
-(*       program_behaves (T.psem (I.get_interface c) (compile (I.link c p))) beh. *)
-(*   Proof. *)
-(*     intros b c p Hcomp H. *)
-(*     destruct (I.link_spec c p (I.link c p) Hcomp) as [Hif [Hvalip Hcompip]]. *)
-(*     destruct (compile_spec (I.link c p)) as [HvalPcom Hcompint]. *)
-(*     unfold I.complete. *)
-(*     split; auto. *)
-(*     apply decomposition. *)
-(*     assumption. *)
-(*     rewrite <- Hcompint. *)
-(*     unfold contained. *)
-(*     exists (I.get_interface p). *)
-(*     auto. *)
-(*     auto. *)
-(*   Qed. *)
+  (* we can prove special decomposition using the more general *)
+  (*      decomposition *)
+  Definition special_decomposition :
+    forall beh (c p:I.program),
+      I.complete2 c p ->
+      let ip := compile (I.link c p) in
+      program_behaves (T.sem ip) beh ->
+      program_behaves (T.psem (I.get_interface c) ip) beh.
+  Proof.
+    intros b c p Hcomp tp H.
+    destruct (I.link_spec c p (I.link c p) Hcomp) as [Hif [Hvalip Hcompip]].
+    destruct (compile_spec (I.link c p)) as [HvalPcom Hcompint].
+    unfold I.complete.
+    split; auto.
+    apply decomposition.
+    assumption.
+    unfold contained.
+    exists (I.get_interface p).
+    rewrite Hcompint in Hif.
+    assumption.
+    assumption.
+  Qed.
 
-(*   (* Note: despite the name this is backward simulation. *)
-(*      In compcert there are two simulation: *)
-(*      - forward: is just a simulation, it is forward or backward depending on the order of the arguments *)
-(*      - backward: add the condition that the first argument must be a safe program *)
-(*   *) *)
-(*   Axiom special_compiler_correctness_simulation: *)
-(*     forall (c p:I.program), *)
-(*       I.complete2 c p -> *)
-(*       I.fully_defined (I.get_interface c) p -> *)
-(*       let ip := I.link c p in *)
-(*       forward_simulation (T.psem (I.get_interface c) (compile ip)) (I.psem (I.get_interface c) p). *)
+  Axiom special_compiler_correctness:
+    forall (beht:program_behavior) (c p:I.program),
+      I.complete2 c p ->
+      let ip := I.link c p in
+      program_behaves (T.psem (I.get_interface c) (compile ip)) beht ->
+      exists behi,
+      program_behaves (I.psem (I.get_interface c) p) behi /\
+      behavior_improves_p behi beht (I.get_interface p).
+End MPC.
 
-(*   Definition special_compiler_correctness: *)
-(*     forall beh (c p:I.program), *)
-(*       I.complete2 c p -> *)
-(*       I.fully_defined (I.get_interface c) p -> *)
-(*       let ip := I.link c p in *)
-(*       program_behaves (T.psem (I.get_interface c) (compile ip)) beh -> *)
-(*       program_behaves (I.psem (I.get_interface c) p) beh. *)
-(*   Proof. *)
-(*     intros b c p Hcompl pFD ip Hcomp. *)
-(*     apply forward_simulation_same_safe_behavior with (L1:=(T.psem (I.get_interface c) (compile ip))). *)
-(*     apply special_compiler_correctness_simulation. *)
-(*     assumption. *)
-(*     assumption. *)
-(*     assumption. *)
-(*     apply (psem_spec (I.get_interface c) (compile ip)). *)
-(*     assumption. *)
-(*   Qed. *)
-(* End MPC. *)
-
-(* (* Software Fault Isolation compiler *) *)
-(* Module SFIC <: IT. *)
-(*   Module T := SFI. *)
+(* Software Fault Isolation compiler *)
+Module SFIC <: IT.
+  Module T := SFI.
   
-(*   Axiom compile : I.program -> T.program. *)
-(*   Axiom compile_spec: *)
-(*     forall (p:I.program), *)
-(*       I.complete p -> T.valid (compile p) /\ *)
-(*                    I.get_interface p = T.get_interface (compile p). *)
+  Axiom compile : I.program -> T.program.
+  Axiom compile_spec:
+    forall (p:I.program),
+      I.complete p -> T.valid (compile p) /\
+                   I.get_interface p = T.get_interface (compile p).
 
-(*   (* Axiom partialize: interface -> T.program -> T.program. *) *)
-(*   (* Axiom partialize_spec: *) *)
-(*   (*   forall psi (p:T.program), *) *)
-(*   (*     T.valid p -> *) *)
-(*   (*     contained psi (T.get_interface p) -> *) *)
-(*   (*     (T.get_interface p) = (T.get_interface (partialize psi p))++psi. *) *)
+  (* Axiom partialize: interface -> T.program -> T.program. *)
+  (* Axiom partialize_spec: *)
+  (*   forall psi (p:T.program), *)
+  (*     T.valid p -> *)
+  (*     contained psi (T.get_interface p) -> *)
+  (*     (T.get_interface p) = (T.get_interface (partialize psi p))++psi. *)
 
-(*   Axiom sem_spec: *)
-(*     forall p b, program_behaves (T.sem p) b -> not_wrong b. *)
+  Axiom sem_spec:
+    forall p b, program_behaves (T.sem p) b -> not_wrong b.
 
-(*   Axiom decomposition_simulation: *)
-(*     forall psi c p, *)
-(*       I.complete2 c p -> *)
-(*       I.fully_defined (I.get_interface c) p -> (* CH: do we really need this? *) *)
-(*       let ip := compile (I.link c p) in *)
-(*       forward_simulation (T.sem ip) (T.psem psi ip). *)
-
-(*   (* there is no generic decomposition, we need to prove *)
-(*       special_decomposition *) *)
-(*   Definition special_decomposition : *)
-(*     forall beh (c p:I.program), *)
-(*       I.complete2 c p -> *)
-(*       I.fully_defined (I.get_interface c) p -> (* CH: do we really need this? *) *)
-(*       let ip := compile (I.link c p) in *)
-(*       program_behaves (T.sem ip) beh -> *)
-(*       program_behaves (T.psem (I.get_interface c) ip) beh. *)
-(*   Proof. *)
-(*     intros b c p Hcompl pFD ip Hsem. *)
-(*     apply (decomposition_simulation (I.get_interface c) c p Hcompl) in pFD. *)
-(*     apply (forward_simulation_same_safe_behavior pFD). *)
-(*     assumption. *)
-(*     apply (sem_spec ip). *)
-(*     assumption. *)
-(*   Qed. *)
+  (* there is no generic decomposition, we need to prove *)
+  (*       special_decomposition *)
+  Axiom special_decomposition :
+    forall beh (c p:I.program),
+      I.complete2 c p ->
+      let ip := compile (I.link c p) in
+      program_behaves (T.sem ip) beh ->
+      program_behaves (T.psem (I.get_interface c) ip) beh.
     
-(*   Axiom special_compiler_correctness: *)
-(*     forall beh (c p:I.program), *)
-(*       I.complete2 c p -> *)
-(*       I.fully_defined (I.get_interface c) p -> *)
-(*       let ip := I.link c p in *)
-(*       program_behaves (T.psem (I.get_interface c) (compile ip)) beh -> *)
-(*       program_behaves (I.psem (I.get_interface c) p)  beh. *)
-(* End SFIC. *)
+  Axiom special_compiler_correctness:
+    forall (beht:program_behavior) (c p:I.program),
+      I.complete2 c p ->
+      let ip := I.link c p in
+      program_behaves (T.psem (I.get_interface c) (compile ip)) beht ->
+      exists behi,
+      program_behaves (I.psem (I.get_interface c) p) behi /\
+      behavior_improves_p behi beht (I.get_interface p).
+End SFIC.
 
 
 
@@ -572,28 +433,31 @@ Module Main (IT : IT).
    semantics by partializing a complete target program.
    *)
 
-  Definition robust_compilation_dynamic_compromise:
+  Definition RC_DC :=
     forall (c:I.program) (P:S.program) (beht:program_behavior),
       I.valid c ->
       S.valid P ->
       icomplete2 (I.get_interface c) (S.get_interface P) ->
-      program_behaves (IT.T.sem (IT.compile (I.link c (SI.compile P)))) beht ->
+      program_behaves (IT.T.sem (IT.compile (I.link c (SI.compile P)))) beht
+      ->
       exists C behs,
         S.valid C /\
         S.get_interface C = I.get_interface c /\
         program_behaves (S.sem (S.link C P)) behs /\
         behavior_improves_p behs beht (S.get_interface P).
+
+  Theorem robust_compilation_dynamic_compromise : RC_DC.
   Proof.
     intros c P bt Hvalc HvalP Hicompl Hsem.
     destruct (SI.compile_spec P HvalP) as [Hvalcomp Hif] .
     apply IT.special_decomposition in Hsem.
-    eapply IT.special_compiler_correctness in Hsem as [H1 H2].
-    apply SI.compiler_correctness in H1.
-    apply S.definability in H1.
-    destruct H1 as [C [H3a [H3b H3c]]].
-    exists C. exists bt.
+    eapply IT.special_compiler_correctness in Hsem as [bi [HPI HimpIT]].
+    apply SI.partial_compiler_correctness in HPI as [bs [HPS HimpSI]].
+    apply S.definability in HPS as [C [HvalC [HCint HCS]]].
+    exists C. exists bs.
     repeat split; eauto.
-    rewrite Hif.
+    rewrite <- Hif in HimpIT.
+    specialize (behavior_improves_p_trans bs bi bt (S.get_interface P) HimpSI HimpIT) as HimpST.
     auto.
     auto.
     auto.
@@ -601,33 +465,32 @@ Module Main (IT : IT).
     auto.
     unfold I.complete2. rewrite <- Hif. repeat split; auto.
     unfold I.complete2. rewrite <- Hif. repeat split; auto.
+Qed.
+
+
+  (* This property is strictly weaker than the above, but has the
+     advantage of not mentioning the intermediate language *)
+  Definition robust_compilation_static_compromise_weaker :=
+    forall (Q P:S.program) (beht:program_behavior),
+      S.complete2 Q P ->
+      program_behaves (IT.T.sem (IT.compile (I.link (SI.compile Q) (SI.compile P)))) beht ->
+      exists C behs,
+        S.valid C /\
+        S.get_interface C = S.get_interface Q /\
+        program_behaves (S.sem (S.link C P)) behs /\
+        behavior_improves_p behs beht (S.get_interface P).
+
+  Corollary robust_compilation_corrolary :
+    RC_DC ->
+    robust_compilation_static_compromise_weaker.
+  Proof.
+    intros RC Q P b Hcompl H2.
+    specialize (RC (SI.compile Q) P b).
+    assert (Hcompl2 := Hcompl).
+    destruct Hcompl2 as [HvalQ [HvalP Hicompl]].
+    destruct (SI.compile_spec Q).
+    auto.
+    rewrite <- H0 in RC.
+    apply (RC H HvalP Hicompl H2).
   Qed.
-
-(* (* This property is strictly weaker than the above, but has the *)
- (*    advantage of not mentioning the intermediate language *) *)
-  (* Definition robust_compilation_static_compromise_weaker := *)
-  (*   forall (Q P:S.program) (beh:program_behavior), *)
-  (*     S.complete2 Q P -> *)
-  (*     S.fully_defined (S.get_interface Q) P -> *)
-  (*     program_behaves (IT.T.sem (IT.compile (I.link (SI.compile Q) (SI.compile P)))) beh -> *)
-  (*     exists C, *)
-  (*       S.valid C /\ *)
-  (*       S.get_interface C = S.get_interface Q /\ *)
-  (*       S.fully_defined (S.get_interface P) C /\  *)
-  (*       program_behaves (S.sem (S.link C P)) beh. *)
-
-  (* Corollary robust_compilation_corrolary : *)
-  (*   robust_compilation_static_compromise -> *)
-  (*   robust_compilation_static_compromise_weaker. *)
-  (* Proof. *)
-  (*   intros RC Q P b Hcompl SFD H2. *)
-  (*   specialize (RC (SI.compile Q) P b). *)
-  (*   assert (SFD2 := SFD). *)
-  (*   assert (Hcompl2 := Hcompl). *)
-  (*   destruct Hcompl2 as [HvalQ [HvalP Hicompl]]. *)
-  (*   destruct (SI.compile_spec Q). *)
-  (*   auto. *)
-  (*   rewrite <- H0 in RC. *)
-  (*   apply (RC H HvalP Hicompl SFD H2). *)
-  (* Qed. *)
 End Main.
